WIP trying to kill remaining admits in poly1305

code/streaming/Hacl.Streaming.Poly1305_32.fst
@@ -39,6 +39,13 @@ let as_lib (x: t): P.poly1305_ctx M32 =
   x
 
 inline_for_extraction noextract
+let k = I.stateful_buffer uint8 32ul (Lib.IntTypes.u8 0)
+
+inline_for_extraction noextract
+let as_lib_k (x: B.buffer uint8 { B.length x = 32 }): Lib.Buffer.lbuffer uint8 32ul =
+  x
+
+inline_for_extraction noextract
 let stateful_poly1305_ctx32: I.stateful unit =
   I.Stateful
     (fun () -> t)
@@ -52,41 +59,6 @@ let stateful_poly1305_ctx32: I.stateful unit =
       P.reveal_ctx_inv (as_lib s) h0 h1;
       B.modifies_buffer_elim (as_raw s) l h0 h1)
     (fun #_ _ _ _ _ -> ())
-
-let update (acc, r) (block: S.seq uint8 { S.length block = Spec.Poly1305.size_block }) =
-  Spec.Poly1305.poly1305_update1 r Spec.Poly1305.size_block block acc, r
-
-inline_for_extraction noextract
-let k = I.stateful_buffer uint8 32
-
-inline_for_extraction noextract
-let as_lib_k (x: B.buffer uint8 { B.length x = 32 }): Lib.Buffer.lbuffer uint8 32ul =
-  x
-
-inline_for_extraction noextract
-let poly1305_32: I.block unit =
-  I.Block
-    I.Runtime
-
-    stateful_poly1305_ctx32
-    k
-
-    (fun () -> pow2 32 - 1)
-    (fun () -> 16ul)
-    (fun () -> 16ul)
-
-    (fun () k -> Spec.Poly1305.poly1305_init k)
-    (fun () acc blocks -> Spec.UpdateMulti.mk_update_multi Spec.Poly1305.size_block update acc blocks)
-    (fun () (acc, r) _ input -> Spec.Poly1305.poly1305_update1 r (S.length input) input acc, r)
-    (fun () k (acc, r) -> Spec.Poly1305.poly1305_finish k acc)
-
-    (fun () k input -> Spec.Poly1305.poly1305_mac input k)
-
-    (fun () -> Spec.UpdateMulti.update_multi_zero Spec.Poly1305.size_block update)
-    (fun () -> Spec.UpdateMulti.update_multi_associative Spec.Poly1305.size_block update)
-    (fun () _ _ -> admit ())
-
-    (fun _ _ -> ())
     (fun () ->
       let h0 = ST.get () in
       let dummy_key = B.alloca (Lib.IntTypes.u8 0) 32ul in
@@ -114,6 +86,128 @@ let poly1305_32: I.block unit =
       B.modifies_only_not_unused_in B.loc_none h0 h3;
       P.reveal_ctx_inv (as_lib r) h2 h3;
       r)
+    (fun _ s -> B.free s)
+    (fun _ src dst ->
+      let h0 = ST.get () in
+      B.blit src 0ul dst 0ul 25ul;
+      let h1 = ST.get () in
+      P.reveal_ctx_inv' (as_lib src) (as_lib dst) h0 h1
+    )
+
+let block = (block: S.seq uint8 { S.length block = Spec.Poly1305.size_block })
+
+let init = Spec.Poly1305.poly1305_init
+
+let update (acc, r) (block: block) =
+  Spec.Poly1305.poly1305_update1 r Spec.Poly1305.size_block block acc, r
+
+let update' r acc (block: block) =
+  Spec.Poly1305.poly1305_update1 r Spec.Poly1305.size_block block acc
+
+let update_multi =
+  Spec.UpdateMulti.mk_update_multi Spec.Poly1305.size_block update
+
+let update_multi' r =
+  Spec.UpdateMulti.mk_update_multi Spec.Poly1305.size_block (update' r)
+
+#push-options "--fuel 1"
+let rec with_or_without_r (acc r: Spec.Poly1305.felem) (blocks: S.seq uint8):
+  Lemma
+    (requires
+      S.length blocks % Spec.Poly1305.size_block = 0)
+    (ensures
+      update_multi (acc, r) blocks == (update_multi' r acc blocks, r))
+    (decreases (S.length blocks))
+=
+  if S.length blocks = 0 then
+    ()
+  else
+    let block, rem = Spec.UpdateMulti.split_block Spec.Poly1305.size_block blocks 1 in
+    let acc = update' r acc block in
+    with_or_without_r acc r rem
+#pop-options
+
+let update_last (acc, r) (input: S.seq uint8 { S.length input < Spec.Poly1305.size_block }) =
+  if S.length input = 0 then
+    acc, r
+  else
+    Spec.Poly1305.poly1305_update1 r (S.length input) input acc, r
+
+let update_last' r acc (input: S.seq uint8 { S.length input < Spec.Poly1305.size_block }) =
+  if S.length input = 0 then
+    acc
+  else
+    Spec.Poly1305.poly1305_update1 r (S.length input) input acc
+
+let finish k (acc, r) =
+  Spec.Poly1305.poly1305_finish k acc
+
+let spec k input =
+  Spec.Poly1305.poly1305_mac input k
+
+val poly_is_incremental:
+  key: S.seq uint8 { S.length key = 32 } ->
+  input:S.seq uint8 { S.length input <= pow2 32 - 1 } ->
+  Lemma (ensures (
+    let open FStar.Mul in
+    let block_length = Spec.Poly1305.size_block in
+    let n = S.length input / block_length in
+    let bs, l = S.split input (n * block_length) in
+    FStar.Math.Lemmas.multiple_modulo_lemma n block_length;
+    let hash = update_multi (init key) bs in
+    let hash = update_last hash l in
+    finish key hash `S.equal` spec key input))
+
+let poly_is_incremental key input =
+  let open Hacl.Streaming.Lemmas in
+  let block_length = Spec.Poly1305.size_block in
+  assert_norm (block_length < pow2 32);
+  let n = S.length input / block_length in
+  let bs, l = S.split input (n * block_length) in
+  FStar.Math.Lemmas.multiple_modulo_lemma n block_length;
+  let acc, r = init key in
+  assume (repeat_f block_length (update' r) == Spec.Poly1305.(poly1305_update1 r size_block));
+  calc (S.equal) {
+    finish key (update_last (update_multi (acc, r) bs) l);
+  (S.equal) { with_or_without_r acc r bs }
+    Spec.Poly1305.poly1305_finish key (update_last' r (update_multi' r acc bs) l);
+  (S.equal) { update_multi_is_repeat_blocks block_length (update' r) (update_last' r) acc input input }
+    Spec.Poly1305.poly1305_finish key (Lib.Sequence.repeat_blocks #uint8 #Spec.Poly1305.felem block_length input
+      (repeat_f block_length (update' r))
+      (repeat_l block_length (update_last' r) input)
+      acc);
+  (S.equal) { }
+    Spec.Poly1305.poly1305_finish key (Lib.Sequence.repeat_blocks #uint8 #Spec.Poly1305.felem block_length input
+      Spec.Poly1305.(poly1305_update1 r size_block)
+      (repeat_l block_length (update_last' r) input)
+      acc);
+  };
+  admit ()
+
+inline_for_extraction noextract
+let poly1305_32: I.block unit =
+  I.Block
+    I.Runtime
+
+    stateful_poly1305_ctx32
+    k
+
+    (fun () -> pow2 32 - 1)
+    (fun () -> 16ul)
+    (fun () -> 16ul)
+
+    (fun () -> init)
+    (fun () x y -> update_multi x y)
+    (fun () x _ y -> update_last x y)
+    (fun () -> finish)
+
+    (fun () -> spec)
+
+    (fun () -> Spec.UpdateMulti.update_multi_zero Spec.Poly1305.size_block update)
+    (fun () -> Spec.UpdateMulti.update_multi_associative Spec.Poly1305.size_block update)
+    (fun () -> poly_is_incremental)
+
+    (fun _ _ -> ())
     (fun _ k s -> P.poly1305_init #M32 s k)
     (fun _ s blocks len -> P.poly1305_update #M32 s len blocks; admit ())
     (fun _ s last total_len ->
@@ -139,11 +233,4 @@ let poly1305_32: I.block unit =
       B.modifies_fresh_frame_popped h0 h1 B.(loc_buffer dst) h4 h5;
       assert B.(loc_disjoint (loc_buffer s) (loc_buffer dst));
       P.reveal_ctx_inv (as_lib s) h0 h5
-    )
-    (fun _ s -> B.free s)
-    (fun _ src dst ->
-      let h0 = ST.get () in
-      B.blit src 0ul dst 0ul 25ul;
-      let h1 = ST.get () in
-      P.reveal_ctx_inv' (as_lib src) (as_lib dst) h0 h1
     )
